\chapter{Modelo lineal General}
\begin{multicols}{2}


$$\beta = \begin{bmatrix}
    \beta_0\\
    \beta_1\\
    \vdots\\
    \beta_n\\
\end{bmatrix}$$

\subsection{Modelo lineal muestral}


\section*{bondad de ajuste}
$Y_i = \hat{Y}_i + e \Longrightarrow ()^2 = (\hat{Y}_i - \overline{Y} + e)^2 \Longrightarrow (Y_i - \overline{Y})^2=(\hat{Y}_i-\overline{Y})^2+2e(\hat{Y}-\overline{Y})^2+e^2 \Longrightarrow \sum\limits_{i=1}^n(Y_i-\overline{Y})^2 = \sum\limits_{i=1}^n (\hat{Y}-\overline{Y})^2 + 2\sum\limits_{i=1}^n e_i (\hat{Y}_i - \overline{Y})+ \sum\limits_{i=1}^n e_i^2$

\end{multicols}

